Struct/CustomTactics.lean
@@ -1,8 +1,17 @@
 import Lean
 
+open
+  Lean.Elab.Tactic
+
 -- Extend tactic version of show to support `by`
 macro "show " type:term " by " tacSeq:tacticSeq : tactic => `(exact show $type by $tacSeq)
 
+
+-- def fix : TacticM Unit := do
+--   let a ← `(tactic|sorry) 
+
+-- elab &"fix " : tactic =>
+--   fix
 
 -- Structured Annotation
 -- `strucNote ($name : $type)* (⊢ $newGoal)? (by $tacSeq)?`
