Struct/Struct.lean
@@ -12,133 +12,166 @@ open
   Lean.Parser 
   Lean.Parser.Tactic
 
+-- TODO: abstract away commonalities between this and other suggestions, like getting goals, extracting info from lCtx
+def structuredIntros (tacSeq : TSyntax ``tacticSeq) (hasExplicitNames : Bool) : TacticM Unit := do
+  addTrace `structured m!"Matched on intro(s), specific implementation"
+  
+  let goal ← getMainGoal
+  let goalType ← instantiateMVars (← goal.getDecl).type
+
+  evalTactic tacSeq
+
+  let newGoal ← getMainGoal
+  let newGoalType ← instantiateMVars (← newGoal.getDecl).type
+
+  let isSameGoal := goalType.consumeMData == newGoalType.consumeMData
+
+  let lCtx := (← goal.getDecl).lctx
+  let lCtxNew := (← newGoal.getDecl).lctx
+
+  let declsNotInNew := diffLCtx lCtx lCtxNew
+  let declsNotInOld := diffLCtx lCtxNew lCtx
+
+  if !isSameGoal ∧ declsNotInNew.size == 0 ∧ declsNotInOld.size > 0 then
+    for decl in declsNotInOld do
+      let bool := decl.userName.isAnonymous
+      addTrace `xx m!"{decl.userName} : {decl.type}, hasExplicitnames: {hasExplicitNames})"
+  else
+    logWarning "Unexpected state in intros match"
+
+#check Name
+
 def structured (tacSeq : TSyntax ``tacticSeq) : TacticM Unit := do
   let tacs ← getTacs tacSeq
 
-  -- TODO : Match
   match tacs with
+  | #[] => logWarning "No tactics in tacSeq"
+  -- TODO: Currently only matching on single tactic, optionally want to allow multiple intro/clear calls
   | #[t] =>
-    addTrace `structured m!"This tactic is already structured"
+    match t with
+    | `(tactic|suffices $_ by $_) 
+    | `(tactic|show $_ by $_) 
+    | `(tactic|have $_ : $_ := by $_) 
+    | `(tactic|clear $_)
+      => 
+      addTrace `structured m!"This tactic is already structured"
+      evalTactic tacSeq
+      return
+    | `(tactic|intro)
+    | `(tactic|intros)
+      =>
+      structuredIntros tacSeq false
+      return
+    | `(tactic|intro $id)
+    | `(tactic|intros $ids*)
+      => 
+      structuredIntros tacSeq true
+      return
+    | `(tactic|cases $target)
+    | `(tactic|induction $target)
+      => 
+      addTrace `structured m!"Matched on cases or induction, specific implementation"
+      evalTactic tacSeq
+      return
+    | _ => pure ()
+  | _ => pure ()
+
+  -- This is executed whenever there is no specific match found above
+  match (← getUnsolvedGoals) with
+  | [] => 
+    logWarning m!"No goals to solve, kind of shouldn't reach this, since we can't execute your tactic anyways"
+  | [goal] => 
+    let goalType ← instantiateMVars (← goal.getDecl).type
     evalTactic tacSeq
-
-  | _ =>
-
-  -- match tacSeq with
-  -- | `(tacticSeq|suffices $_ by $_) 
-  -- | `(tacticSeq|show $_ by $_) 
-  -- | `(tacticSeq|have $_ : $_ := by $_) 
-  -- | `(tacticSeq|clear $_)
-  --   => 
-  --   addTrace `structured m!"This tactic is already structured"
-  --   evalTactic tacSeq
-  -- | `(tacticSeq|intro)
-  -- | `(tacticSeq|intro $id)
-  -- | `(tacticSeq|intros)
-  -- | `(tacticSeq|intros $ids*)
-  --   =>
-  --   addTrace `structured m!"Matched with intro, currently unimplemented"
-  --   evalTactic tacSeq
-  -- | `(tacticSeq|cases $_)
-  -- | `(tacticSeq|induction $_)
-  --   => 
-  --   addTrace `structured m!"Matched with cases or induction, currently unimplemented"
-  --   evalTactic tacSeq
-  -- | _ => 
     match (← getUnsolvedGoals) with
     | [] => 
-      logWarning m!"No goals to solve, kind of shouldn't reach this, since we can't execute your tactic anyways"
-    | [goal] => 
-      let goalType ← instantiateMVars (← goal.getDecl).type
-      evalTactic tacSeq
-      match (← getUnsolvedGoals) with
-      | [] => 
-        let goalStx ← delab goalType
-        let stx ← mkShow goalStx tacSeq
+      let goalStx ← delab goalType
+      let stx ← mkShow goalStx tacSeq
+      addTrace `structured m!"Try this: {stx}"
+    | [newGoal] => 
+      let newGoalType ← instantiateMVars (← newGoal.getDecl).type
+      let isSameGoal := goalType.consumeMData == newGoalType.consumeMData
+
+      let lCtx := (← goal.getDecl).lctx
+      let lCtxNew := (← newGoal.getDecl).lctx
+
+      let declsNotInNew := diffLCtx lCtx lCtxNew
+      let declsNotInOld := diffLCtx lCtxNew lCtx
+
+      if !isSameGoal && declsNotInNew.size = 0 && declsNotInOld.size = 0 then
+        let newGoalStx ← delab (← instantiateMVars newGoalType)
+        let stx ← mkSuffices newGoalStx tacSeq
         addTrace `structured m!"Try this: {stx}"
-      | [newGoal] => 
-        let newGoalType ← instantiateMVars (← newGoal.getDecl).type
-        let isSameGoal := goalType.consumeMData == newGoalType.consumeMData
+      else if h : isSameGoal ∧ declsNotInNew.size = 0 ∧ declsNotInOld.size = 1 then
+        -- Prove that we know we can use the first index
+        have : 0 < declsNotInOld.size := by simp_all
+        let decl := declsNotInOld[0]
+        let declStx ← delab decl.type
+        -- NOTE: this stx does not really make sense, because from what I understand it can only happen if there is already a have clause
+        let newStx ← mkHave declStx tacSeq
+        addTrace `structured m!"Try this: {newStx}"
+      else
+        -- temp investigating types
+        -- let lCtx : LocalContext := (← goal.getDecl).lctx
+        -- for (decl : LocalDecl) in lCtx do
+        --   addTrace `structured m!"Decl Type : {decl.type}"
 
-        let lCtx := (← goal.getDecl).lctx
-        let lCtxNew := (← newGoal.getDecl).lctx
+        --   -- Something with ConstantInfo, inductInfo
 
-        let declsNotInNew := diffLCtx lCtx lCtxNew
-        let declsNotInOld := diffLCtx lCtxNew lCtx
+        --   -- REALLY hacky way of ensuring we have the right decl we want to find constructors of
+        --   if toString decl.type == "Nat" then
+        --     let t : Expr := decl.type
+        --     addTrace `structured m!"Type Expression : {t}"
+        --     addTrace `structured m!"Expression Constructor : {Lean.Expr.ctorName t}"
+        --     match t with
+        --     | .const n us =>
+        --       addTrace `structured m!"Expression construcion with name : {n} and us {us}"
+        --       let x := (← getEnv).find? n
+        --       match x with 
+        --       | some (.inductInfo ival) => 
+        --         let ctors := ival.ctors
+        --       | _ => return
 
-        if !isSameGoal && declsNotInNew.size = 0 && declsNotInOld.size = 0 then
-          let newGoalStx ← delab (← instantiateMVars newGoalType)
-          let stx ← mkSuffices newGoalStx tacSeq
-          addTrace `structured m!"Try this: {stx}"
-        else if h : isSameGoal ∧ declsNotInNew.size = 0 ∧ declsNotInOld.size = 1 then
-          -- Prove that we know we can use the first index
-          have : 0 < declsNotInOld.size := by simp_all
-          let decl := declsNotInOld[0]
-          let declStx ← delab decl.type
-          -- NOTE: this stx does not really make sense, because from what I understand it can only happen if there is already a have clause
-          let newStx ← mkHave declStx tacSeq
-          addTrace `structured m!"Try this: {newStx}"
-        else
-          -- temp investigating types
-          -- let lCtx : LocalContext := (← goal.getDecl).lctx
-          -- for (decl : LocalDecl) in lCtx do
-          --   addTrace `structured m!"Decl Type : {decl.type}"
+        --     | _ =>
+        --       addTrace `structured m!"other"
 
-          --   -- Something with ConstantInfo, inductInfo
+            -- TODO: how to get the existing known constructors of the const Nat
+            
+            -- Borrowed from Ed Ayers, but is not a match statement, doesnt use info on the type
+            -- let stx ← `(tactic| cases $(TSyntax.mk <| mkIdent localDecl.userName))
 
-          --   -- REALLY hacky way of ensuring we have the right decl we want to find constructors of
-          --   if toString decl.type == "Nat" then
-          --     let t : Expr := decl.type
-          --     addTrace `structured m!"Type Expression : {t}"
-          --     addTrace `structured m!"Expression Constructor : {Lean.Expr.ctorName t}"
-          --     match t with
-          --     | .const n us =>
-          --       addTrace `structured m!"Expression construcion with name : {n} and us {us}"
-          --       let x := (← getEnv).find? n
-          --       match x with 
-          --       | some (.inductInfo ival) => 
-          --         let ctors := ival.ctors
-          --       | _ => return
+        -- end
+        logWarning m!"That combination of changes in goals and local declarations is currently unsupported 
+                      isSameGoal: {isSameGoal} {goalType} {newGoalType}
+                      NotInNew: {declsNotInNew.size} {declsNotInNew.map (fun x => x.type)} 
+                      NotInOld: {declsNotInOld.size} {declsNotInOld.map (fun x => x.type)}"
 
-          --     | _ =>
-          --       addTrace `structured m!"other"
+    | newGoals => 
+      logWarning m!"Multiple goals after tactic execution, TODO to implement a case distinction suggestion"
+      -- temp for investigating case autocomplete
+      -- let mut cases := #[]
 
-              -- TODO: how to get the existing known constructors of the const Nat
-              
-              -- Borrowed from Ed Ayers, but is not a match statement, doesnt use info on the type
-              -- let stx ← `(tactic| cases $(TSyntax.mk <| mkIdent localDecl.userName))
+      -- for newGoal in newGoals do
+      --   let tag ← newGoal.getTag
+      --   let tseq ← `(tacticSeq|sorry)
+      --   let caseStx ← `(tactic|
+      --     case $(TSyntax.mk <| mkIdent tag):ident =>
+      --       $tseq:tacticSeq)
+      --   cases := cases.push caseStx
+      
+      -- -- TODO: Find neat way of unpacking cases
+      -- -- let firstCase := $cases[0]!
+      -- -- let allStx ← `(tacticSeq|
+      -- --   $tacSeq;
+      -- --   $firstCase)
 
-          -- end
-          logWarning m!"That combination of changes in goals and local declarations is currently unsupported 
-                        isSameGoal: {isSameGoal} {goalType} {newGoalType}
-                        NotInNew: {declsNotInNew.size} {declsNotInNew.map (fun x => x.type)} 
-                        NotInOld: {declsNotInOld.size} {declsNotInOld.map (fun x => x.type)}"
+      -- addTrace `structured m!"All Case Syntax combined : TODO"
+      -- -- end temp
 
-      | newGoals => 
-        logWarning m!"Multiple goals after tactic execution, TODO to implement a case distinction suggestion"
-        -- temp for investigating case autocomplete
-        -- let mut cases := #[]
-
-        -- for newGoal in newGoals do
-        --   let tag ← newGoal.getTag
-        --   let tseq ← `(tacticSeq|sorry)
-        --   let caseStx ← `(tactic|
-        --     case $(TSyntax.mk <| mkIdent tag):ident =>
-        --       $tseq:tacticSeq)
-        --   cases := cases.push caseStx
-        
-        -- -- TODO: Find neat way of unpacking cases
-        -- -- let firstCase := $cases[0]!
-        -- -- let allStx ← `(tacticSeq|
-        -- --   $tacSeq;
-        -- --   $firstCase)
-
-        -- addTrace `structured m!"All Case Syntax combined : TODO"
-        -- -- end temp
-
-    | goal::moreGoals =>
-      let goalDecl ← goal.getDecl
-      logWarning m!"Multiple goals pre-execution. This tactic may not work as expected if multiple goals change. Currently unimplemented"
-      evalTactic tacSeq
+  | goal::moreGoals =>
+    let goalDecl ← goal.getDecl
+    logWarning m!"Multiple goals pre-execution. This tactic may not work as expected if multiple goals change. Currently unimplemented"
+    evalTactic tacSeq
 
 -- Elaborate tactic
 elab &"structured " t:tacticSeq : tactic =>
